trying simple wp_rec example

Concrete.v
@@ -4,44 +4,77 @@ From iris.proofmode Require Export tactics.
 From iris.heap_lang Require Import proofmode notation.
 Set Default Proof Using "Type".
 
-Definition incrementer (l : expr) : expr := l <- !l + #1.
+Section Concrete.
+  Context `{heapG Σ}.
 
-Lemma simple_assign `{!heapG Σ} l (n : Z):
-  [[{ l ↦ #n }]]
-    incrementer #l
-  [[{ RET #(); l ↦ #(n + 1) }]].
-Proof.
-  iIntros (Φ) "Hloc HΦ".
-  rewrite /incrementer.
-  wp_load.
-  wp_store.
-  by iApply "HΦ".
-Qed.
+  Definition incrementer (l : expr) : expr := l <- !l + #1.
 
-Check simple_assign.
+  Lemma simple_assign l (n : Z):
+    [[{ l ↦ #n }]]
+      incrementer #l
+      [[{ RET #(); l ↦ #(n + 1) }]].
+  Proof.
+    iIntros (Φ) "Hloc HΦ".
+    rewrite /incrementer.
+    wp_load.
+    wp_store.
+    by iApply "HΦ".
+  Qed.
 
-(* Questions/remarks: *)
+  Check simple_assign.
 
-(* The Σ here in the type of simple_assign is determined by Coq, presumably by looking for a type that matches the typeclass constraint heapG? *)
+  (* Questions/remarks: *)
 
-(* Compared to the lecture notes, there seems to be no need to invoke a "wp_bind" rule for getting to the right part of an evaluation context. We can just use wp_load and wp_store right away. *)
+  (* The Σ here in the type of simple_assign is determined by Coq, presumably by looking for a type that matches the typeclass constraint heapG? *)
 
-(* Unset Printing Notations. *)
+  (* Compared to the lecture notes, there seems to be no need to invoke a "wp_bind" rule for getting to the right part of an evaluation context. We can just use wp_load and wp_store right away. *)
 
-Lemma simple_assign2 `{!heapG Σ} l (n : Z):
-  [[{ l ↦ #n }]]
-    (incrementer #l);; (incrementer #l)
-  [[{ RET #(); l ↦ #(n + 2) }]].
-Proof.
-  iIntros (Φ) "Hloc HΦ".
-  (* wp_seq. *)
-  wp_apply (simple_assign with "Hloc").
-  iIntros "Hloc2".
-  wp_seq.
-  wp_apply (simple_assign with "Hloc2").
-  iIntros "Hloc3".
-  iApply "HΦ".
-  replace (n + 1 + 1) with (n + 2).
-  - done.
-  - omega.
-Qed.
+  (* Unset Printing Notations. *)
+
+  Lemma simple_assign2 l (n : Z):
+    [[{ l ↦ #n }]]
+      (incrementer #l);; (incrementer #l)
+      [[{ RET #(); l ↦ #(n + 2) }]].
+  Proof.
+    iIntros (Φ) "Hloc HΦ".
+    (* wp_seq. *)
+    wp_apply (simple_assign with "Hloc").
+    iIntros "Hloc".
+    wp_seq.
+    wp_apply (simple_assign with "Hloc").
+    iIntros "Hloc".
+    iApply "HΦ".
+    replace (n + 1 + 1) with (n + 2).
+    - done.
+    - omega.
+  Qed.
+
+  (* loop n = if n = 0 then 0 else loop (n - 1) + 1
+
+  This is simply the identity function for non-negative integers,
+  implemented in a roundabout fashion. *)
+  Definition simple_loop : val :=
+    rec: "loop" "n" :=
+      if: "n" = #0
+      then #0
+      else "loop" ("n" - #1) + #1.
+
+  (* The error message you get when you forget the heapG Σ is somewhat
+  cryptic. I just put it in the Context now so I cannot forget
+  anymore. *)
+
+  (* If I make simple_loop an expr then wp_rec (understandably) fails
+  to work with a cryptic error message. Presumably I have to "reduce"
+  the left-hand side of the application to a value first. *)
+
+  Lemma spec_simple_loop (n : nat):
+    WP simple_loop #n {{ v, ⌜v = #n⌝}}%I.
+  Proof.
+    iInduction n as [|n'] "IH"; rewrite /simple_loop; wp_rec.
+    - wp_op. wp_if_true. done.
+    - wp_op. wp_if_false. wp_op.
+      assert (Hn': S n' - 1 = n'). { admit. }
+      rewrite Hn'.
+  Admitted.
+
+End Concrete.
